src/ssa/opsem_pp.v
@@ -1,0 +1,607 @@
+Add LoadPath "./ott".
+Add LoadPath "./monads".
+Add LoadPath "../../../theory/metatheory".
+Require Import ssa_mem.
+Require Import genericvalues.
+Require Import ssa_dynamic.
+Require Import ssa.
+Require Import trace.
+Require Import List.
+Require Import tactics.
+Require Import Coq.Program.Equality.
+Require Import CoqListFacts.
+Require Import Bool.
+Require Import Metatheory.
+
+Export LLVMsyntax.
+Export LLVMlib.
+Export LLVMopsem.
+
+(* eq *)
+
+Lemma blockEqB_refl : forall B,
+  blockEqB B B.
+Admitted.
+     
+Lemma productEqB_refl : forall p,
+  productEqB p p.
+Admitted.
+
+Lemma blockEqB_inv : forall B1 B2,
+  blockEqB B1 B2 -> B1 = B2.
+Admitted.
+
+Lemma moduleEqB_inv : forall M M',
+  moduleEqB M M' ->
+  M = M'.
+Admitted.
+
+Lemma productEqB_inv : forall P P',
+  productEqB P P' ->
+  P = P'.
+Admitted.
+
+
+(* prop *)
+
+Lemma getIncomingValuesForBlockFromPHINodes_eq : forall ps l1 ps1 cs1 tmn1 ps2 cs2 tmn2,
+  getIncomingValuesForBlockFromPHINodes ps (block_intro l1 ps1 cs1 tmn1) =
+  getIncomingValuesForBlockFromPHINodes ps (block_intro l1 ps2 cs2 tmn2).
+Proof.
+  induction ps; intros; auto.
+    simpl.
+    erewrite IHps; eauto.
+Qed.
+
+Lemma switchToNewBasicBlock_eq : forall B l1 ps1 cs1 tmn1 ps2 cs2 tmn2 lc,
+  switchToNewBasicBlock B (block_intro l1 ps1 cs1 tmn1) lc =
+  switchToNewBasicBlock B (block_intro l1 ps2 cs2 tmn2) lc.
+Proof.
+  intros.
+  unfold switchToNewBasicBlock.
+  erewrite getIncomingValuesForBlockFromPHINodes_eq; eauto.
+Qed.
+
+Lemma dbop_trans : forall state1 state2 state3 tr1 tr2,
+  dbop state1 state2 tr1 ->
+  dbop state2 state3 tr2 ->
+  dbop state1 state3 (trace_app tr1 tr2).
+Proof.
+  intros state1 state2 state3 tr1 tr2 H.
+  generalize dependent state3.
+  generalize dependent tr2.
+  induction H; intros; auto.
+    rewrite <- trace_app_commute. eauto.
+Qed.
+
+Lemma dbInsn__dbop : forall state1 state2 tr,
+  dbInsn state1 state2 tr ->
+  dbop state1 state2 tr.
+Proof.
+  intros.
+  rewrite <- trace_app_nil__eq__trace.
+  eapply dbop_cons; eauto.
+Qed.
+
+Lemma dbInsn__inv : forall S1 TD1 Ps1 F1 l1 ps1 cs1 tmn1 c cs tmn3 lc1 arg1 als1 ECs1 gl1 Mem1
+                         S2 TD2 Ps2 F2 l2 ps2 cs2 tmn2 tmn4 lc2 arg2 als2 ECs2 gl2 Mem2 tr,
+  dbInsn 
+    (mkState S1 TD1 Ps1 (mkEC F1 (block_intro l1 ps1 cs1 tmn1) (c::cs) tmn3 lc1 arg1 als1::ECs1) gl1 Mem1) 
+    (mkState S2 TD2 Ps2 (mkEC F2 (block_intro l2 ps2 cs2 tmn2) cs tmn4 lc2 arg2 als2::ECs2) gl2 Mem2)
+    tr ->
+  S1 = S2 /\ TD1 = TD2 /\ Ps1 = Ps2 /\ F1 = F2 /\ l1 = l2 /\ ps1 = ps2 /\
+  cs1 = cs2 /\ tmn1 = tmn2 /\ tmn3 = tmn4.
+Proof.
+  intros.
+  inversion H; subst; repeat (split; auto).
+Qed.
+
+Lemma dbInsn_Call__inv : forall S1 TD1 Ps1 F1 l1 ps1 cs1 tmn1 c cs tmn3 lc1 arg1 als1 ECs1 gl1 Mem1
+                         S2 TD2 Ps2 F2 l2 ps2 cs2 tmn2 tmn4 lc2 arg2 als2 ECs2 gl2 Mem2 tr,
+  
+  dbInsn 
+    (mkState S1 TD1 Ps1 (mkEC F1 (block_intro l1 ps1 cs1 tmn1) (c::cs) tmn3 lc1 arg1 als1::ECs1) gl1 Mem1) 
+    (mkState S2 TD2 Ps2 (mkEC F2 (block_intro l2 ps2 cs2 tmn2) cs tmn4 lc2 arg2 als2::ECs2) gl2 Mem2)
+    tr ->
+  Instruction.isCallInst c = true ->
+  S1 = S2 /\ TD1 = TD2 /\ Ps1 = Ps2 /\ F1 = F2 /\ l1 = l2 /\ ps1 = ps2 /\
+  cs1 = cs2 /\ tmn1 = tmn2 /\ tmn3 = tmn4 /\ als1 = als2.
+Proof.
+  intros.
+  inversion H; subst; try solve [inversion H0].
+    repeat (split; auto).
+Qed.
+
+Lemma InBlocksB_middle : forall lb1 B lb2,
+  InBlocksB B (lb1++B::lb2).
+Proof.
+  induction lb1; intros; simpl; auto.
+    apply orb_true_intro.
+    left. apply blockEqB_refl.
+
+    apply orb_true_intro.
+    right. apply IHlb1.
+Qed. 
+
+Lemma _genLabel2Block_blocks_inv : forall lb2 lb1 lb f l0 l' ps' cs' tmn',
+  genLabel2Block_blocks lb2 (fdef_intro f lb) l0 = Some (block_intro l' ps' cs' tmn') ->
+  lb1++lb2 = lb ->
+  l0 = l' /\
+  blockInFdefB (block_intro l' ps' cs' tmn') (fdef_intro f lb).
+Proof.
+  induction lb2; intros; simpl in *.
+    inversion H.
+
+    unfold mergel2block in H.
+    remember (genLabel2Block_blocks lb2 (fdef_intro f lb) l0) as ob.
+    destruct ob.
+      inversion H; subst. clear H.
+      symmetry in Heqob.
+      apply IHlb2 with (lb1:=lb1++a::nil) in Heqob; simpl_env; auto.
+       
+      unfold genLabel2Block_block in H.
+      destruct a.
+      destruct (l0 == l1); subst.
+        inversion H; subst. clear H.
+        split; auto using InBlocksB_middle.
+
+        inversion H.
+Qed.
+
+Lemma genLabel2Block_blocks_inv : forall lb f l0 l' ps' cs' tmn',
+  genLabel2Block_blocks lb (fdef_intro f lb) l0 = Some (block_intro l' ps' cs' tmn') ->
+  l0 = l' /\
+  blockInFdefB (block_intro l' ps' cs' tmn') (fdef_intro f lb).
+Proof.
+  intros.
+  apply _genLabel2Block_blocks_inv with (lb1:=nil)(lb2:=lb); auto.
+Qed.
+
+
+Lemma lookupBlockViaLabelFromFdef_inv : forall F l0 l' ps' cs' tmn',
+  lookupBlockViaLabelFromFdef F l0 = Some (block_intro l' ps' cs' tmn') ->
+  l0 = l' /\
+  blockInFdefB (block_intro l' ps' cs' tmn') F.
+Proof.
+  intros.
+  unfold lookupBlockViaLabelFromFdef in H.
+  unfold genLabel2Block_fdef in H.
+  destruct F.
+  apply genLabel2Block_blocks_inv; auto.
+Qed. 
+
+Lemma lookupFdefViaIDFromProducts_inv : forall Ps fid F,
+  lookupFdefViaIDFromProducts Ps fid = Some F ->
+  InProductsB (product_fdef F) Ps.
+Proof.
+  induction Ps; intros.
+    simpl in H. inversion H.
+
+    simpl in *.
+    unfold lookupFdefViaIDFromProduct in H.
+    destruct a.
+      apply IHPs in H. auto.
+      apply IHPs in H. auto.
+      destruct (getFdefID f==fid); subst.
+        inversion H; subst.
+        apply orb_true_intro.
+        left. apply productEqB_refl.
+
+        apply IHPs in H. 
+        apply orb_true_intro. auto.
+Qed.
+
+Lemma entryBlockInFdef : forall F B,
+  getEntryBlock F = Some B ->
+  blockInFdefB B F.
+Proof.
+  intros.
+  unfold getEntryBlock in H.
+  destruct F.
+  destruct b; inversion H; subst.
+    simpl. 
+    apply orb_true_intro.
+    left. apply blockEqB_refl.
+Qed.
+
+Lemma blockInSystemModuleFdef_inv : forall B F Ps TD S,
+  blockInSystemModuleFdef B S (module_intro TD Ps) F ->
+  blockInFdefB B F /\
+  InProductsB (product_fdef F) Ps /\
+  moduleInSystem (module_intro TD Ps) S /\
+  productInSystemModuleB (product_fdef F) S (module_intro TD Ps).
+Proof.
+  intros.
+  unfold blockInSystemModuleFdef in H.
+  unfold blockInSystemModuleFdefB in H.
+  unfold productInSystemModuleB in *.
+  unfold productInModuleB in *.
+  apply andb_true_iff in H. destruct H.
+  split; auto.
+  apply andb_true_iff in H0. destruct H0.
+  split; auto.
+  split; auto.
+  eapply andb_true_iff.
+  split; auto.
+Qed.
+
+Lemma blockInSystemModuleFdef_intro : forall B F Ps TD S,
+  blockInFdefB B F ->
+  InProductsB (product_fdef F) Ps ->
+  moduleInSystem (module_intro TD Ps) S ->
+  blockInSystemModuleFdef B S (module_intro TD Ps) F.
+Proof.
+  intros.
+  unfold blockInSystemModuleFdef.
+  unfold blockInSystemModuleFdefB.
+  unfold productInSystemModuleB.
+  unfold productInModuleB.
+  eapply andb_true_iff.
+  split; auto.
+  eapply andb_true_iff.
+  split; auto.
+Qed.  
+
+Lemma entryBlockInSystemBlockFdef : forall TD Ps S fid F B,
+  moduleInSystem (module_intro TD Ps) S ->
+  lookupFdefViaIDFromProducts Ps fid = Some F ->
+  getEntryBlock F = Some B ->
+  blockInSystemModuleFdef B S (module_intro TD Ps) F.
+Proof.
+  intros.
+  apply lookupFdefViaIDFromProducts_inv in H0.
+  apply entryBlockInFdef in H1.
+  apply blockInSystemModuleFdef_intro; auto.
+Qed.
+
+Lemma NotIn_NotInBlocksB : forall lb l0 ps cs tmn,
+  ~ In l0 (getBlocksLabels lb) ->
+  ~ InBlocksB (block_intro l0 ps cs tmn) lb.
+Proof.
+  induction lb; intros; simpl in *.
+    intro J. inversion J.
+
+    destruct a.
+    simpl in *.
+    remember (block_intro l0 ps cs tmn =b= block_intro l1 p c t) as J.
+    destruct J.
+      unfold blockEqB in HeqJ.
+      unfold lEqB in HeqJ.
+      destruct (l0==l1); subst.
+        contradict H; auto.
+        inversion HeqJ.
+
+      intro J.
+      apply H.
+      right.
+      apply orb_prop in J.
+      destruct J as [J | J].
+        inversion J.
+     
+        destruct (@In_dec _ eq_dec l0 (getBlocksLabels lb)) as [J1 | J1]; auto.
+        apply IHlb with (ps:=ps)(cs:=cs)(tmn:=tmn) in J1.
+        rewrite J in J1.
+        contradict J1; auto.
+        unfold is_true. auto.
+Qed.
+
+Lemma InBlocksB_In : forall lb l0 ps cs tmn,
+  InBlocksB (block_intro l0 ps cs tmn) lb ->
+  In l0 (getBlocksLabels lb).
+Proof.
+  intros.
+  destruct (@In_dec _ eq_dec l0 (getBlocksLabels lb)) as [J1 | J1]; auto.
+    apply NotIn_NotInBlocksB with (ps:=ps)(cs:=cs)(tmn:=tmn) in J1.
+    contradict H; auto.
+Qed.
+
+Lemma NoDup_split : forall A (l1 l2:list A),
+  NoDup (l1++l2) ->
+  NoDup l1 /\ NoDup l2.
+Proof.
+  induction l1; intros.
+    simpl in *. 
+    split; auto using NoDup_nil.
+ 
+    inversion H; subst.
+    apply IHl1 in H3.
+    destruct H3 as [J1 J2].
+    split; auto.
+      apply NoDup_cons; auto.
+        intro J. apply H2. apply in_or_app; auto.
+Qed.
+
+Lemma InBlocksB_uniq : forall lb l1 ps1 cs1 tmn1 ps2 cs2 tmn2,
+  uniqBlocks lb ->
+  InBlocksB (block_intro l1 ps1 cs1 tmn1) lb ->
+  InBlocksB (block_intro l1 ps2 cs2 tmn2) lb ->
+  ps1 = ps2 /\ cs1 = cs2 /\ tmn1 = tmn2.
+Proof.
+  induction lb; intros.
+    unfold InBlocksB in *.
+    inversion H0.
+
+    inversion H; subst. clear H.
+    simpl in *.
+    destruct a.
+    inversion H2; subst. clear H2.
+    assert (J:=H5).
+    apply NotIn_NotInBlocksB with (ps:=p)(cs:=c)(tmn:=t) in H5.
+    apply orb_prop in H0.
+    apply orb_prop in H1.
+    destruct H0 as [H0 | H0].    
+      apply blockEqB_inv in H0.
+      inversion H0; subst. clear H0.
+      destruct H1 as [H1 | H1].
+        apply blockEqB_inv in H1.
+        inversion H1; subst. clear H1.
+        auto.
+
+        apply InBlocksB_In in H1.
+        contradict H1; auto.
+ 
+      destruct H1 as [H1 | H1].
+        apply blockEqB_inv in H1.
+        inversion H1; subst. clear H1.
+        apply InBlocksB_In in H0.
+        contradict H0; auto.
+
+        eapply IHlb; eauto.
+          apply NoDup_split in H3.
+          destruct H3.
+          split; auto.
+Qed.
+
+Lemma blockInFdefB_uniq : forall l1 ps1 cs1 tmn1 ps2 cs2 tmn2 F,
+  uniqFdef F ->
+  blockInFdefB (block_intro l1 ps1 cs1 tmn1) F ->
+  blockInFdefB (block_intro l1 ps2 cs2 tmn2) F ->
+  ps1 = ps2 /\ cs1 = cs2 /\ tmn1 = tmn2.
+Proof.
+  intros.
+  unfold blockInFdefB in *.
+  destruct F.
+  eapply InBlocksB_uniq; eauto.
+Qed.
+
+Lemma blockInSystemModuleFdef_uniq : forall l1 ps1 cs1 tmn1 ps2 cs2 tmn2 S M F,
+  uniqFdef F ->
+  blockInSystemModuleFdef (block_intro l1 ps1 cs1 tmn1) S M F ->
+  blockInSystemModuleFdef (block_intro l1 ps2 cs2 tmn2) S M F ->
+  ps1 = ps2 /\ cs1 = cs2 /\ tmn1 = tmn2.
+Proof.
+  intros.
+  unfold blockInSystemModuleFdef in *.
+  unfold blockInSystemModuleFdefB in *.
+  apply andb_true_iff in H0.
+  apply andb_true_iff in H1.
+  destruct H0.
+  destruct H1.
+  eapply blockInFdefB_uniq; eauto.
+Qed.
+
+Lemma uniqProducts__uniqFdef : forall Ps F,
+  uniqProducts Ps ->
+  InProductsB (product_fdef F) Ps ->
+  uniqFdef F.
+Proof.
+  induction Ps; intros.
+    inversion H0.
+    
+    simpl in *.
+    destruct H.
+    apply orb_prop in H0.
+    destruct H0; eauto.
+      apply productEqB_inv in H0. subst.
+      simpl in H. auto.
+Qed.
+
+Lemma uniqSystem__uniqFdef : forall S F M,
+  uniqSystem S ->
+  productInSystemModuleB (product_fdef F) S M ->
+  uniqFdef F.
+Proof.
+  induction S; intros.
+    unfold productInSystemModuleB in H0.
+    apply andb_true_iff in H0.
+    destruct H0.
+    unfold moduleInSystemB in H0.
+    inversion H0.
+
+    unfold productInSystemModuleB in H0.
+    apply andb_true_iff in H0.
+    destruct H0.
+    unfold moduleInSystemB in H0.
+    inversion H0. clear H0.
+    apply orb_prop in H3.
+    simpl in H.
+    destruct H as [J1 J2].
+    destruct H3 as [H3 | H3].
+      apply moduleEqB_inv in H3. subst.
+      destruct a.
+      simpl in H1. simpl in J1. destruct J1.
+      eapply uniqProducts__uniqFdef; eauto.
+
+      apply IHS with (M:=M); auto.
+        unfold productInSystemModuleB.
+        eapply andb_true_iff; auto.
+Qed.
+
+(* preservation *)
+
+Definition dbInsn_preservation_prop state1 state2 tr
+  (db:dbInsn state1 state2 tr) :=
+  forall S TD Ps F l ps cs tmn lc arg als ECs gl Mem cs0,
+  state1 = (mkState S TD Ps ((mkEC F (block_intro l ps cs0 tmn) cs tmn lc arg als)::ECs) gl Mem) ->
+  blockInSystemModuleFdef (block_intro l ps cs0 tmn) S (module_intro TD Ps) F ->
+  exists l', exists ps', exists cs', exists tmn', 
+  exists lc', exists als', exists gl', exists Mem', exists cs0',
+  state2 = (mkState S TD Ps ((mkEC F (block_intro l' ps' cs0' tmn') cs' tmn' lc' arg als')::ECs) gl' Mem') /\
+  blockInSystemModuleFdef (block_intro l' ps' cs0' tmn') S (module_intro TD Ps) F.
+Definition dbop_preservation_prop state1 state2 tr
+  (db:dbop state1 state2 tr) :=
+  forall S TD Ps F l ps cs tmn lc arg als ECs gl Mem l' ps' cs' tmn' lc' als' gl' Mem' cs0 cs0',
+  state1 = (mkState S TD Ps ((mkEC F (block_intro l ps cs0 tmn) cs tmn lc arg als)::ECs) gl Mem) ->
+  state2 = (mkState S TD Ps ((mkEC F (block_intro l' ps' cs0' tmn') cs' tmn' lc' arg als')::ECs) gl' Mem') ->
+  blockInSystemModuleFdef (block_intro l ps cs0 tmn) S (module_intro TD Ps) F ->
+  blockInSystemModuleFdef (block_intro l' ps' cs0' tmn') S (module_intro TD Ps) F.
+Definition dbFdef_preservation_prop fid rt lp S TD Ps ECs lc gl Mem lc' gl' als' Mem' B' Rid oResult tr
+  (db:dbFdef fid rt lp S TD Ps ECs lc gl Mem lc' gl' als' Mem' B' Rid oResult tr) :=
+  moduleInSystem (module_intro TD Ps) S ->
+  exists F, 
+    lookupFdefViaIDFromProducts Ps fid = Some F /\
+    blockInSystemModuleFdef B' S (module_intro TD Ps) F.
+
+Lemma db_preservation : 
+  (forall state1 state2 tr db, @dbInsn_preservation_prop state1 state2 tr db) /\
+  (forall state1 state2 tr db, @dbop_preservation_prop state1 state2 tr  db) /\
+  (forall fid rt lp S TD Ps lc gl Mem lc' gl' als' Mem' B' Rid oResult tr ECs db, 
+    @dbFdef_preservation_prop fid rt lp S TD Ps lc gl Mem lc' gl' als' Mem' B' Rid oResult tr ECs db).
+Proof.
+(db_mutind_cases
+  apply LLVMopsem.db_mutind with
+    (P  := dbInsn_preservation_prop)
+    (P0 := dbop_preservation_prop)
+    (P1 := dbFdef_preservation_prop) Case);
+  unfold dbInsn_preservation_prop, 
+         dbop_preservation_prop, 
+         dbFdef_preservation_prop; intros; subst;
+  try solve [
+  inversion H; subst;
+  exists l0; exists ps; exists cs; exists tmn0;
+  exists lc'; exists als0; exists gl'; exists Mem1;
+  exists cs1; split; auto
+    ].
+Case "dbBranch".
+  inversion H; subst. clear H.
+  exists l'. exists ps'. exists cs'. exists tmn'.
+  exists (switchToNewBasicBlock (block_intro l' ps' cs' tmn') (block_intro l0 ps cs0 (insn_br bid Cond l1 l2)) lc0). exists als0. exists gl0. exists Mem1.
+  exists cs'. split; auto.
+  apply andb_true_iff in H0.
+  destruct H0.
+  eapply andb_true_iff.
+  split; auto.
+    symmetry in e0.
+    destruct c;
+      apply lookupBlockViaLabelFromFdef_inv in e0;
+      destruct e0; auto.
+
+Case "dbBranch_uncond".
+  inversion H; subst. clear H.
+  exists l'. exists ps'. exists cs'. exists tmn'.
+  exists (switchToNewBasicBlock (block_intro l' ps' cs' tmn') (block_intro l1 ps cs0 (insn_br_uncond bid l0)) lc0). exists als0. exists gl0. exists Mem1.
+  exists cs'. split; auto.
+  apply andb_true_iff in H0.
+  destruct H0.
+  eapply andb_true_iff.
+  split; auto.
+    symmetry in e.
+    apply lookupBlockViaLabelFromFdef_inv in e.
+    destruct e; auto.
+
+Case "dbMalloc".
+  inversion H; subst.
+  exists l0. exists ps. exists cs. exists tmn0.
+  exists lc'. exists als0. exists gl'. exists Mem'.
+  exists cs1. split; auto.
+
+Case "dbFree".
+  inversion H; subst. 
+  exists l0. exists ps. exists cs. exists tmn0.
+  exists lc0. exists als0. exists gl0. exists Mem'.
+  exists cs1. split; auto.
+
+Case "dbAlloca".
+  inversion H; subst. 
+  exists l0. exists ps. exists cs. exists tmn0.
+  exists lc'. exists (mb::als0). exists gl'. exists Mem'.
+  exists cs1. split; auto.
+
+Case "dbStore".
+  inversion H; subst. 
+  exists l0. exists ps. exists cs. exists tmn0.
+  exists lc0. exists als0. exists gl0. exists Mem'.
+  exists cs1. split; auto.
+
+Case "dbCall".
+  inversion H0; subst. clear H0.
+  exists l0. exists ps. exists cs. exists tmn0.
+  exists lc''. exists als0. exists gl''. exists Mem''.
+  exists cs1. split; auto.
+ 
+Case "dbop_nil".
+  inversion H0; subst. auto.
+  
+Case "dbop_cons".
+  apply H with (cs1:=cs)(lc0:=lc)(arg:=arg0)(als0:=als)(ECs0:=ECs)(gl0:=gl)(Mem:=Mem0) in H3; auto.
+  clear H.
+  destruct H3 as [l1 [ps1 [cs1 [tmn1 [lc1 [als1 [gl1 [Mem1 [cs1' [EQ H3]]]]]]]]]]; subst.
+  eapply H0; eauto.
+
+Case "dbFdef_func".
+  exists (fdef_intro (fheader_intro rt fid la) lb).
+  split; auto.
+    eapply H; eauto using entryBlockInSystemBlockFdef.
+
+Case "dbFdef_proc".
+  exists (fdef_intro (fheader_intro rt fid la) lb).
+  split; auto.
+    eapply H; eauto using entryBlockInSystemBlockFdef.
+Qed.
+
+Lemma _dbInsn_preservation : forall state2 tr S TD Ps F l ps cs tmn lc arg als ECs gl Mem cs0,
+  dbInsn ((mkState S TD Ps ((mkEC F (block_intro l ps cs0 tmn) cs tmn lc arg als)::ECs) gl Mem)) state2 tr ->
+  blockInSystemModuleFdef (block_intro l ps cs0 tmn) S (module_intro TD Ps) F ->
+  exists l', exists ps', exists cs', exists tmn', 
+  exists lc', exists als', exists gl', exists Mem', exists cs0',
+  state2 = (mkState S TD Ps ((mkEC F (block_intro l' ps' cs0' tmn') cs' tmn' lc' arg als')::ECs) gl' Mem') /\
+  blockInSystemModuleFdef (block_intro l' ps' cs0' tmn') S (module_intro TD Ps) F.
+Proof.
+  intros.
+  destruct db_preservation as [J _].
+  unfold dbInsn_preservation_prop in J.
+  eapply J; eauto.
+Qed.
+
+Lemma dbInsn_preservation : forall tr S TD Ps F l ps cs tmn lc arg als ECs gl Mem cs0
+  l' ps'  cs' tmn' lc' als' gl' Mem' cs0',
+  dbInsn 
+    ((mkState S TD Ps ((mkEC F (block_intro l ps cs0 tmn) cs tmn lc arg als)::ECs) gl Mem)) 
+    (mkState S TD Ps ((mkEC F (block_intro l' ps' cs0' tmn') cs' tmn' lc' arg als')::ECs) gl' Mem')
+    tr ->
+  blockInSystemModuleFdef (block_intro l ps cs0 tmn) S (module_intro TD Ps) F ->
+  blockInSystemModuleFdef (block_intro l' ps' cs0' tmn') S (module_intro TD Ps) F.
+Proof.
+  intros.
+  apply _dbInsn_preservation in H; auto.
+  destruct H as [l1 [ps1 [cs1 [tmn1 [lc1 [als1 [gl1 [Mem1 [cs2 [J1 J2]]]]]]]]]].
+  inversion J1; subst. clear J1. auto.  
+Qed.
+
+Lemma dbop_preservation : forall tr S TD Ps F l ps cs tmn lc arg als ECs gl Mem l' ps' cs' tmn' lc' als' gl' Mem' cs0 cs0',
+  dbop 
+    (mkState S TD Ps ((mkEC F (block_intro l ps cs0 tmn) cs tmn lc arg als)::ECs) gl Mem)
+    (mkState S TD Ps ((mkEC F (block_intro l' ps' cs0' tmn') cs' tmn' lc' arg als')::ECs) gl' Mem')
+    tr ->
+  blockInSystemModuleFdef (block_intro l ps cs0 tmn) S (module_intro TD Ps) F ->
+  blockInSystemModuleFdef (block_intro l' ps' cs0' tmn') S (module_intro TD Ps) F.
+Proof.
+  intros.
+  destruct db_preservation as [_ [J _]].
+  unfold dbop_preservation_prop in J.
+  eapply J; eauto.
+Qed.
+
+Lemma dbFdef_preservation : forall fid rt lp S TD Ps ECs lc gl Mem lc' gl' als' Mem' B' Rid oResult tr,
+  dbFdef fid rt lp S TD Ps ECs lc gl Mem lc' gl' als' Mem' B' Rid oResult tr ->
+  moduleInSystem (module_intro TD Ps) S ->
+  exists F, 
+    lookupFdefViaIDFromProducts Ps fid = Some F /\
+    blockInSystemModuleFdef B' S (module_intro TD Ps) F.
+Proof.
+  intros.
+  destruct db_preservation as [_ [_ J]].
+  unfold dbFdef_preservation_prop in J.
+  eapply J; eauto.
+Qed.
+
